src/util/meta/expr.lean
@@ -28,4 +28,10 @@ meta def expr.is_mvar : expr → bool
 meta def expr.list_meta_vars (e : expr) : list expr :=
 e.fold [] (λ e' _ es, if expr.is_mvar e' ∧ ¬ e' ∈ es then e' :: es else es)
 
+meta def expr.list_const (e : expr) : list expr :=
+e.fold [] (λ e' _ es, if expr.is_constant e' ∧ ¬ e' ∈ es then e' :: es else es)
+
+meta def expr.list_local_const (e : expr) : list expr :=
+e.fold [] (λ e' _ es, if expr.is_local_constant e' ∧ ¬ e' ∈ es then e' :: es else es)
+
 end expr
